ETCSList.sml
@@ -5,7 +5,8 @@ if l is in in the set, then for every a\in A, l ∪ (CARD l,a) is in the set
 
 *)
 
- 
+
+
 val Lists_cond_ex = prove_store("Lists_cond_ex",
 e0
 (rpt strip_tac >> 
@@ -16,22 +17,527 @@ e0
  >> rw[o_assoc,Pa_distr,IN_def] >>
  once_rw[one_to_one_id] >> rw[idL,idR,True1TRUE]) >>
  pop_assum strip_assume_tac >>
+ qsuff_tac
+ ‘?P1. !ls. P1 o ls = TRUE <=> 
+ (!l:1-> Exp(N * A,1+1). IN(l,ls) ==>
+ !a. IN(Ins(Pa(CARD(l),a),l), ls))’ >-- 
+ (strip_tac >>
+ qexists_tac ‘And(P0,P1)’ >>
+ once_rw[GSYM And_def] >> once_rw[o_assoc] >>
+ once_rw[Pa_distr] >> 
+ once_rw[CONJ_def] >> arw[]) >>
+ pop_assum (K all_tac) >>
+ qsuff_tac
+ ‘?P2. !l ls. P2 o Pa(l,ls) = TRUE <=> 
+  (IN(l,ls) ==>
+   !a:1->A. IN(Ins(Pa(CARD(l),a),l), ls))’ >--
+ (strip_tac >> qexists_tac ‘ALL(P2)’ >>
+  once_rw[GSYM ALL_def] >> once_rw[o_assoc] >>
+  once_rw[All_def] >> arw[]) >>
  qby_tac
- ‘?P1. !a:1->A l ls.
-    P1 o Pa(a,Pa(l,ls)) = TRUE<=>
-    !n. hasCard(ls,n) ==> 
- !a. IN(Ins(Pa(n,a),l), ls)’ >-- 
-(qexists_tac
- ‘Mem(Exp(N * A, 1 + 1)) o 
-  Pa(Ins(
-     Pa
-     (CARD
-      (p32(A,Exp(N * A, 1 + 1),Exp(Exp(N * A, 1 + 1),1+1))), 
-      p31(A,Exp(N * A, 1 + 1),Exp(Exp(N * A, 1 + 1),1+1))),
-     p32(A,Exp(N * A, 1 + 1),Exp(Exp(N * A, 1 + 1),1+1))),
+ ‘?P3. !l:1-> Exp(N * A,1+1) ls. P3 o Pa(l,ls) = TRUE <=> 
+  IN(l,ls)’
+ >-- (qexists_tac ‘Mem(Exp(N * A,1+1))’ >>
+      rw[IN_def,True1TRUE]) >>
+ pop_assum strip_assume_tac >> 
+ qsuff_tac
+ ‘?P4. !a l:1-> Exp(N * A,1+1) ls.
+ P4 o Pa(a,Pa(l,ls)) = TRUE <=> 
+ IN(Ins(Pa(CARD(l),a),l), ls)’ 
+ >-- (strip_tac >> 
+      qexists_tac ‘Imp(P3,ALL(P4))’ >>
+      once_rw[GSYM Imp_def] >> once_rw[o_assoc] >>
+      once_rw[Pa_distr] >> once_rw[IMP_def] >>
+      rw[ALL_property] >> arw[]) >>
+ pop_assum (K all_tac) >>
+ rw[IN_def,True1TRUE] >>
+ qexists_tac ‘ Mem(Exp(N * A, 1 + 1)) o Pa(Ins(
+ Pa
+ (CARD(p32(A,Exp(N * A,1+1),Exp(Exp(N * A, 1 + 1), 1 + 1)))
+ ,
+ p31(A,Exp(N * A,1+1),Exp(Exp(N * A, 1 + 1), 1 + 1))
+  )
+  ,
+ p32(A,Exp(N * A,1+1),Exp(Exp(N * A, 1 + 1), 1 + 1)))
+ ,
+ p33(A,Exp(N * A,1+1),Exp(Exp(N * A, 1 + 1), 1 + 1))
 )
+’ >>
+ rw[Pa3_def,GSYM Ins_def] >> rw[Pa_distr,o_assoc] >>
+ rw[p31_of_Pa3,p32_of_Pa3,p33_of_Pa3] >>
+ once_rw[GSYM CARD_def] >> rw[o_assoc,Pa_distr] >>
+ once_rw[p32_of_Pa3] >> rw[])
 (form_goal “!A.?P. !ls.P o ls = TRUE <=>
 IN(Empty(N * A),ls) &
  !l. IN(l,ls) ==>
- !n. hasCard(ls,n) ==> 
- !a. IN(Ins(Pa(n,a),l), ls)”)
+ !a. IN(Ins(Pa(CARD(l),a),l), ls)”));
+
+(*sets contain the set of lists as a subset*)
+val cLists_def = Lists_cond_ex |>  spec_all
+                               |> ex2fsym0 "cLists" ["A"]
+                               |> gen_all
+                               |> store_as "cLists_def";
+
+val Lists_ex = prove_store("Lists_ex",
+e0
+(strip_tac >> qexists_tac ‘BIGINTER(Exp(N * A,1+1)) o 
+           Tp1(cLists(A))’ >> rw[])
+(form_goal
+ “!A. ?la. BIGINTER(Exp(N * A,1+1)) o 
+           Tp1(cLists(A)) = la”));
+
+val Lists_def = Lists_ex |> spec_all |> ex2fsym0 "Lists" ["A"]
+                           |> gen_all
+                           |> store_as "Lists_def";
+
+val isList_ex = prove_store("isList_ex",
+e0
+(strip_tac >> qexists_tac ‘Tp0(Lists(A))’ >> rw[])
+(form_goal “!A. ?isl. Tp0(Lists(A)) = isl”));
+
+
+val isList_def = isList_ex |> spec_all |> ex2fsym0 "isList" ["A"]
+                           |> gen_all
+                           |> store_as "isList_def";
+
+val isList_property = prove_store("isList_property",
+e0
+(rpt strip_tac >> once_rw[GSYM isList_def] >>
+ once_rw[GSYM Lists_def] >> 
+ once_rw[GSYM Tp0_def] >> once_rw[o_assoc] >>
+ once_rw[Pa_distr] >> rw[o_assoc,idL] >>
+ once_rw[one_to_one_id] >> rw[idR] >>
+ rw[BIGINTER_property] >> 
+ rw[GSYM Tp1_def] >> rw[Ev_of_Tp_el',p12_of_Pa,o_assoc] >>
+ rw[Ev_of_el] >> 
+ once_rw[cLists_def] >> rw[IN_o] >>
+ dimp_tac >> rpt strip_tac (* 2 *)
+ >-- (first_x_assum (qspecl_then [‘Tp1(P)’] assume_tac) >>
+     fs[Tp0_Tp1_inv] >> rfs[]) >>
+ last_x_assum (qsspecl_then [‘Tp0(s0)’] assume_tac) >> rfs[]
+)
+(form_goal
+ “!A l. isList(A) o l = TRUE <=> 
+  (!P.( P o Empty(N * A) = TRUE &
+      (!l0. P o l0 = TRUE ==>
+        !a. P o Ins(Pa(CARD(l0),a),l0) = TRUE)) ==> 
+      P o l = TRUE)”));
+
+val List_def = pred_subset_ex' 
+                 |> sspecl [rastt "isList(A)"]
+                 |> ex2fsym0 "List" ["A"]
+                 |> ex2fsym0 "LI" ["A"]
+                 |> gen_all
+                 |> store_as "List_def";
+
+val List_def1= List_def |> spec_all |> conjE2
+                        |> allE ONE
+                        |> rewr_rule[True1TRUE]
+                        |> gen_all
+                        |> store_as "List_def1";
+
+val isList_Empty = prove_store("isList_Empty",
+e0
+(rw[isList_property] >> rpt strip_tac >> arw[])
+(form_goal
+ “!A. isList(A) o Empty(N * A) = TRUE”));
+
+val isList_cons = prove_store("isList_cons",
+e0
+(rw[isList_property] >> rpt strip_tac >>
+ first_x_assum (qspecl_then [‘P’] assume_tac) >> rfs[] >>
+ first_x_assum irule >> arw[])
+(form_goal
+ “!A l. isList(A) o l = TRUE ==> 
+  !a. isList(A) o Ins(Pa(CARD(l),a),l) = TRUE”));
+
+val Nil_ex = prove_store("Nil_ex",
+e0
+(rw[GSYM List_def,isList_Empty,True1TRUE])
+(form_goal
+ “!A.?nil:1->List(A). Empty(N * A) = LI(A) o nil”));
+
+val Nil_def = Nil_ex |> spec_all |> ex2fsym0 "Nil" ["A"]
+                     |> gen_all
+                     |> GSYM
+                     |> store_as "Nil_def";
+
+val Cons_rel_ex = prove_store("Cons_ex",
+e0
+(strip_tac >> qexists_tac 
+ ‘Eq(Exp(N * A,1+1)) o Pa(
+  Ins(
+      Pa(
+         CARD(LI(A) o p2(A,List(A)) o p1(A * List(A),List(A)))
+         , 
+         p1(A,List(A)) o p1(A * List(A),List(A)))
+      , 
+      LI(A) o p2(A,List(A)) o p1(A * List(A),List(A)))
+  ,
+  LI(A) o p2(A * List(A),List(A)))’ >>
+ rw[o_assoc] >> rw[Pa_distr] >> rw[Eq_property_TRUE] >>
+ rw[o_assoc] >> rw[p12_of_Pa] >>
+ rw[GSYM Ins_def,o_assoc,p12_of_Pa,Pa_distr] >>
+ rw[GSYM CARD_def,o_assoc,p12_of_Pa,Pa_distr])
+(form_goal
+ “!A. ?R: (A * List(A)) * List(A) -> 1+1.
+ !a0 l0 l. R o Pa(Pa(a0,l0),l) = TRUE <=> 
+ Ins(Pa(CARD(LI(A) o l0),a0),LI(A) o l0) = LI(A) o l ”));
+
+val Crel_def = Cons_rel_ex |> spec_all |> ex2fsym0 "Crel" ["A"]
+                           |> gen_all 
+                           |> store_as "Crel_def";
+
+val Cons_ex = prove_store("Cons_ex",
+e0
+(strip_tac >>
+ assume_tac Rel2Ar' >>
+ first_x_assum (qsspecl_then [‘Crel(A)’] assume_tac) >>
+ qby_tac
+ ‘!al:1-> A * List(A). ?!l. Crel(A) o Pa(al,l) = TRUE’
+ >-- (strip_tac >> uex_tac >> 
+      qsspecl_then [‘al’] (x_choosel_then ["a0","l0"] assume_tac)
+      has_components >>
+      fs[] >> rw[Crel_def] >>
+      qby_tac ‘isList(A) o (LI(A) o l0) = TRUE’
+      >-- (rw[List_def1] >> qexists_tac ‘l0’ >> rw[]) >>
+      drule isList_cons  >>
+      first_x_assum (qspecl_then [‘a0’] assume_tac) >>
+      drule $ iffLR List_def1 >>
+      pop_assum (x_choosel_then ["l"] assume_tac) >>
+      qexists_tac ‘l’ >> arw[] >>
+      rpt strip_tac >> irule $ iffLR Mono_def >>
+      qexistsl_tac [‘Exp(N * A,1+1)’,‘LI(A)’] >> arw[List_def]) >>
+ first_x_assum drule >>
+ pop_assum (x_choosel_then ["cons"] assume_tac) >>
+ qexists_tac ‘cons’ >> arw[] >> 
+ rw[Crel_def])
+(form_goal
+ “!A. ?cons:A * List(A) ->List(A). 
+  !a0:1->A l0 l:1->List(A). cons o Pa(a0,l0) = l <=> 
+  Ins(Pa(CARD(LI(A) o l0),a0),LI(A) o l0) = LI(A) o l”));
+
+val Cons_def = Cons_ex |> spec_all |> ex2fsym0 "Cons" ["A"]
+                       |> gen_all
+                       |> store_as "Cons_def";
+
+
+val cRf_ex = prove_store("Rf_ex",
+e0
+(rpt strip_tac >>
+ qby_tac
+ ‘?P0. !ss. P0 o ss = TRUE <=> IN(Pa(Nil(A), x), ss)’
+ >-- (qexists_tac 
+     ‘Mem(List(A) * X) o Pa(Pa(Nil(A), x) o To1(Exp(List(A) * X,1+1)),
+      id(Exp(List(A) * X,1+1)))’
+      >> rw[IN_def1] >> rw[o_assoc,Pa_distr,idL] >>
+      once_rw[one_to_one_id] >> rw[idR]) >>
+ pop_assum strip_assume_tac >> 
+ qsuff_tac
+ ‘?P1. !ss. P1 o ss = TRUE <=> 
+  !l x. IN(Pa(l, x), ss) ==>
+  !a. IN(Pa(Cons(A) o Pa(a, l), t o Pa(a, x)), ss)’ 
+ (*here if forgot strip the P0, so P0 is not in context, still be able to qexists on CONJ o Pa(P0,P1), check this*)
+ >-- (strip_tac >> qexists_tac ‘CONJ o Pa(P0,P1)’ >> 
+      arw[o_assoc,Pa_distr,CONJ_def]) >>
+ qsuff_tac
+ ‘?P2. !x:1->List(A) l ss. 
+  P2 o Pa(x,Pa(l,ss)) = TRUE <=>
+   IN(Pa(l, x), ss) ==>
+  !a:1->A. IN(Pa(Cons(A) o Pa(a, l), t o Pa(a, x)), ss)’
+ >-- (strip_tac >>
+      qexists_tac ‘ALL(ALL(P2))’ >>
+      rw[ALL_property] >> arw[]) >>
+ qby_tac
+ ‘?P3. !x:1->X l:1->List(A) ss.
+  P3 o Pa(x,Pa(l,ss)) = TRUE <=> IN(Pa(l,x),ss)’
+ >-- (qexists_tac 
+     ‘Mem(List(A) * X) o 
+      Pa(Pa(p32(X,List(A),Exp(List(A) * X,1+1)),
+            p31(X,List(A),Exp(List(A) * X,1+1))), p33(X,List(A),Exp(List(A) * X,1+1)))’ >>
+     rw[Pa3_def,o_assoc,Pa_distr,
+       p31_of_Pa3,p32_of_Pa3,p33_of_Pa3] >> rw[GSYM IN_def1]) >>
+ pop_assum strip_assume_tac >> 
+ qsuff_tac
+ ‘?P4. !a:1->A x:1->X l:1->List(A) ss. 
+  P4 o Pa4(a,x,l,ss) = TRUE <=>
+  IN(Pa(Cons(A) o Pa(a, l), t o Pa(a, x)), ss)’
+ >-- (strip_tac >> qexists_tac ‘Imp(P3,ALL(P4))’ >>
+      rw[GSYM Imp_def,o_assoc,Pa_distr,IMP_def] >>
+      arw[] >>
+      arw[ALL_property,Pa4_def]) >>
+ qexists_tac ‘
+ Mem(List(A) * X) o Pa(
+Pa (CONS(p41(A,X,List(A),Exp(List(A) * X,1+1)),
+    p43(A,X,List(A),Exp(List(A) * X,1+1)))
+    ,
+    t o Pa(p41(A,X,List(A),Exp(List(A) * X,1+1)),
+           p42(A,X,List(A),Exp(List(A) * X,1+1))))
+,
+ p44(A,X,List(A),Exp(List(A) * X,1+1))
+)’ >>
+ rw[GSYM CONS_def,o_assoc,Pa_distr,
+    p41_of_Pa4,p42_of_Pa4,p43_of_Pa4,p44_of_Pa4] >>
+ rw[GSYM IN_def1])
+(form_goal
+ “!X x:1->X A t:A * X ->X.
+  ?P:Exp(List(A) * X,1+1) -> 1 + 1.
+  !ss. P o ss = TRUE <=> 
+       IN(Pa(Nil(A), x),ss) & 
+       (!l:1-> List(A) x:1->X. IN(Pa(l,x),ss) ==> 
+             !a. IN(Pa(Cons(A) o Pa(a,l), t o Pa(a,x)),ss) )”));
+
+val cRf_def = cRf_ex |> spec_all |> ex2fsym0 "cRf" ["x","t"]
+                     |> qgen ‘t’ |> qgen ‘A’
+                     |> gen_all 
+                     |> store_as "cRf_def";
+
+val Rf_ex = prove_store("Rf_ex",
+e0
+(rpt strip_tac >> 
+ qexists_tac ‘Tp0(BIGINTER(List(A) * X) o Tp1(cRf(x,t)))’ >> rw[])
+(form_goal
+ “!X x:1->X A t:A * X ->X.
+  ?R.Tp0(BIGINTER(List(A) * X) o Tp1(cRf(x,t))) = R”));
+
+val Rf_def = Rf_ex |> spec_all |> ex2fsym0 "Rf" ["x","t"]
+                   |> qgen ‘t’ |> qgen ‘A’
+                   |> gen_all 
+                   |> store_as "Rf_def";
+
+val CONS_ex = prove_store("CONS_ex",
+e0
+(rpt strip_tac >> qexists_tac ‘Cons(A) o Pa(a0,l0)’ >> rw[])
+(form_goal
+ “!X a0:X->A l0. ?l. Cons(A) o Pa(a0,l0) = l”));
+
+val CONS_def = CONS_ex |> spec_all |> ex2fsym0 "CONS" ["a0","l0"]
+                       |> gen_all |> store_as "CONS_def";
+
+
+val isList_ind =
+    isList_property |> iffLR
+                    |> strip_all_and_imp
+                    |> disch “isList(A) o l = TRUE”
+                    |> gen_all
+                    |> disch_all |> gen_all
+                    |> store_as "isList_ind";
+
+val LI_Mono = List_def |> spec_all |> conjE1
+                       |> gen_all
+                       |> store_as "LI_Mono";
+
+
+val List_ind = prove_store("List_ind",
+e0
+(assume_tac isList_ind >> rpt strip_tac >>
+ qby_tac
+ ‘?P0:Exp(N * A,1+1) -> 1+1.
+  !ss. P0 o ss = TRUE <=>
+  ?l:1->List(A). ss = LI(A) o l & P o l = TRUE’
+ >-- (qexists_tac 
+      ‘EX(And(Eq(Exp(N * A,1+1)) o 
+              Pa(p2(List(A), Exp(N * A,1+1)),
+                 LI(A) o p1(List(A), Exp(N * A,1+1))) ,
+              P o p1(List(A), Exp(N * A,1+1))))’ >>
+      rw[EX_property] >>
+      rw[GSYM And_def,o_assoc,Pa_distr,p12_of_Pa] >>
+      rw[CONJ_def,Eq_property_TRUE]) >>
+ pop_assum strip_assume_tac >>
+ qsuff_tac 
+ ‘P0 o LI(A) o l = TRUE’ 
+ >-- (arw[] >> rpt strip_tac >>
+      qsuff_tac ‘l = l'’ >-- (strip_tac >> arw[]) >>
+      qspecl_then [‘A’] assume_tac LI_Mono >>
+      drule $ iffLR Mono_def >> first_x_assum drule >>
+      arw[]) >>
+ first_assum irule >> rw[List_def1] >> strip_tac (* 2 *)
+ >-- (qexists_tac ‘l’ >> rw[]) >>
+ arw[] >> rpt strip_tac (* 2 *)
+ >-- (qexists_tac ‘Nil(A)’ >> arw[Nil_def]) >>
+ qexists_tac ‘CONS(a,l')’ >> first_assum drule >> arw[] >>
+ rw[GSYM Cons_def] >> rw[GSYM CONS_def]
+ )
+(form_goal
+ “!A P. P o Nil(A) = TRUE & 
+        (!l. P o l = TRUE ==> !a. P o CONS(a,l) = TRUE) ==>
+        !l. P o l = TRUE”));
+
+
+val Rf_property = prove_store("Rf_property",
+e0
+(once_rw[GSYM Rf_def] >> 
+ once_rw[GSYM Tp0_def] >> once_rw[o_assoc] >>
+ once_rw[Pa_distr] >> once_rw[o_assoc] >>
+ once_rw[idL] >> once_rw[one_to_one_id] >>
+ once_rw[idR] >> once_rw[BIGINTER_property] >>
+ once_rw[GSYM Tp1_def] >>
+ once_rw[Ev_of_Tp_el'] >> once_rw[o_assoc] >>
+ once_rw[p1_of_Pa] >> once_rw[Mem_def] >> once_rw[GSYM IN_def1] >>
+ once_rw[cRf_def] >> once_rw[CONS_def] >> rpt strip_tac >>
+ first_assum irule >> first_assum irule >> arw[])
+(form_goal
+ “!X x:1->X A t:A * X ->X. Rf(x,t) o Pa(Nil(A),x) = TRUE & 
+   !l x0. Rf(x,t) o Pa(l,x0) = TRUE ==> 
+   !a. Rf(x,t) o Pa(CONS(a,l), t o Pa(a,x0)) = TRUE
+  ”));
+
+
+
+
+
+val Rf_min = prove_store("Rf_min",
+e0
+(once_rw[GSYM Rf_def] >> 
+ once_rw[GSYM Tp0_def] >> once_rw[o_assoc] >>
+ once_rw[Pa_distr] >> once_rw[o_assoc] >>
+ once_rw[idL] >> once_rw[one_to_one_id] >>
+ once_rw[idR] >> once_rw[BIGINTER_property] >>
+ once_rw[GSYM Tp1_def] >>
+ once_rw[Ev_of_Tp_el'] >> once_rw[o_assoc] >>
+ once_rw[p1_of_Pa] >> once_rw[Mem_def] >> once_rw[GSYM IN_def1] >>
+ once_rw[cRf_def]  >> rpt strip_tac >>
+ first_x_assum (qsspecl_then [‘Tp1(P)’] assume_tac) >>
+ fs[IN_o,Tp0_Tp1_inv] >>
+ first_assum irule >> arw[CONS_def])
+(form_goal
+ “!X x:1->X A t:A * X ->X P. P o Pa(Nil(A),x) = TRUE & 
+   (!l x0. P o Pa(l,x0) = TRUE ==> 
+          !a. P o Pa(CONS(a,l), t o Pa(a,x0)) = TRUE) ==> 
+   !l x0. Rf(x,t) o Pa(l,x0) = TRUE ==> P o Pa(l,x0) = TRUE
+  ”));
+
+val CONS_NOTNIL = prove_store("CONS_NOTNIL",
+e0
+(rpt strip_tac >> ccontra_tac >>
+ fs[GSYM CONS_def,Cons_def,Nil_def] >> 
+ fs[Ins_NONEMPTY])
+(form_goal
+ “!A a l. ~(CONS(a,l) = Nil(A))”));
+
+val Rf_Nil_unique = prove_store("Rf_base_unique",
+e0
+(rpt strip_tac >> ccontra_tac >> 
+ qsuff_tac ‘?P. P o Pa(Nil(A),x) = TRUE & 
+   (!l x0. P o Pa(l,x0) = TRUE ==> 
+    !a. P o Pa(CONS(a,l), t o Pa(a,x0)) = TRUE) & 
+    ~(P o Pa(Nil(A),x0) = TRUE)’ >--
+ (strip_tac >>
+  qsspecl_then [‘x’,‘t’,‘P’] assume_tac Rf_min>>
+  qby_tac ‘P o Pa(Nil(A), x0) = TRUE’
+  >-- (first_x_assum irule>> arw[]) >>
+  fs[]) >>
+ qsuff_tac
+ ‘?P. !l1 x1. P o Pa(l1,x1) = TRUE <=> 
+  Rf(x,t) o Pa(l1,x1) = TRUE & ~(l1 = Nil(A) & x1 = x0)’
+ >-- (strip_tac >> qexists_tac ‘P’ >>
+      arw[] >> strip_tac (* 2 *)
+      >-- (rw[Rf_property] >> dflip_tac >> arw[]) >>
+      (*should not need the thing between the rpt strip ans fs. should be done by arw*)
+      rpt strip_tac >> fs[] >>
+      first_assum (qsspecl_then [‘l’,‘x0'’] assume_tac) >> 
+      fs[] >>
+      qsspecl_then [‘x’,‘t’] strip_assume_tac Rf_property >>
+      last_x_assum (K all_tac) >>
+      first_x_assum rev_drule >> arw[] >>
+      rw[CONS_NOTNIL]) >>
+ qexists_tac
+ ‘And(Rf(x,t),
+      Not
+      (And(Eq(List(A)) o 
+           Pa(p1(List(A),X),Nil(A) o To1(List(A) * X)),
+           Eq(X) o 
+           Pa(p2(List(A),X), x0 o To1(List(A) * X)) )))’ >>
+ rw[GSYM And_def] >> once_rw[o_assoc] >>
+ once_rw[Pa_distr] >> once_rw[CONJ_def] >>
+ once_rw[GSYM Not_def] >> once_rw[o_assoc] >>
+ once_rw[NEG_def] >> once_rw[o_assoc] >>
+ once_rw[Pa_distr] >> rw[TRUE_xor_FALSE] >> once_rw[CONJ_def] >>
+ rw[o_assoc,Pa_distr] >> once_rw[one_to_one_id] >>
+ rw[idR,p12_of_Pa] >> rw[Eq_property_TRUE])
+(form_goal
+ “!X x:1->X A t:A * X ->X x0. Rf(x,t) o Pa(Nil(A),x0) = TRUE ==> x0 = x”));
+
+
+val Rf_CONS = Rf_property |> spec_all |> conjE2
+                          |> gen_all
+                          |> store_as "Rf_CONS";
+
+val CONS_eq_eq = prove_store("CONS_eq_eq",
+e0
+(strip_tac >>
+ qby_tac
+ ‘?P. !a’)
+(form_goal
+ “!A a1:1->A l1:1->List(A) a2 l2.
+  CONS(a1,l1) = CONS(a2,l2) <=> (a1 = a2 & l2 = l2) ”));
+
+
+val Rf_Cons_back = prove_store("Rf_Cons_back",
+e0
+(strip_tac >> strip_tac >> strip_tac >> strip_tac >>
+ qby_tac
+ ‘?P. !l0:1->List(A) x0:1->X. P o Pa(l0,x0) = TRUE <=>
+  (Rf(x,t) o Pa(l0,x0) = TRUE & 
+  !a:1->A l1. l0 = CONS(a,l1) ==> 
+  ?x1:1->X. Rf(x,t) o Pa(l1,x1) = TRUE & x0 = t o Pa(a,x1))’
+ >-- cheat >>
+ pop_assum strip_assume_tac >>
+ qsuff_tac
+ ‘!l0 x0.Rf(x, t) o Pa(l0, x0) = TRUE ==> P o Pa(l0,x0) = TRUE’
+ >-- (rpt strip_tac >> first_x_assum drule >> rfs[] >>
+      first_x_assum drule >> arw[]) >>
+ match_mp_tac Rf_min >> arw[] >> 
+ rw[GSYM CONS_NOTNIL] >> rpt strip_tac (* 3 *)
+ >-- rw[Rf_property] 
+ >-- (drule Rf_CONS >> arw[]) >>
+ cases_on
+ “?a2:1->A l2. l = CONS(a2,l2)”
+ >-- (pop_assum strip_assume_tac >> first_x_assum drule >>
+      pop_assum strip_assume_tac >>  
+      qby_tac ‘l1 = l’ >-- cheat
+      (*need lemma saying a:: l = a' :: l'*) >>
+      qexists_tac ‘x0'’ >> arw[] >> fs[] >> 
+      qby_tac ‘a = a'’ >-- cheat >> arw[]) >>
+ (*need lemma saying cons xor nil,so if it is not cons, then it is nil*)
+ qby_tac ‘l = Nil(A)’ >-- cheat >> fs[] >>
+ qby_tac ‘l1 = l’ >-- cheat >> fs[] >>
+ qexists_tac ‘x0'’ >> fs[] >>
+ qby_tac ‘a = a'’ >-- cheat >> arw[] 
+)
+(form_goal
+ “!X x:1->X A t:A * X ->X l0 x0. Rf(x,t) o Pa(l0,x0) = TRUE ==>
+  Rf(x,t) o Pa(l0,x0) = TRUE & 
+  !a l1. l0 = CONS(a,l1) ==> 
+  ?x1. Rf(x,t) o Pa(l1,x1) = TRUE & x0 = t o Pa(a,x1)”));
+
+val Rf_unique = prove_store("Rf_unique",
+e0
+(strip_tac >> strip_tac >> strip_tac >> strip_tac >> 
+ qby_tac
+ ‘?P. !l0 x0. P o Pa(l0,x0) = TRUE <=>
+ (!x'. Rf(x,t) o Pa(l0,x') = TRUE ==> x' = x0)’
+ >-- cheat >> pop_assum strip_assume_tac >>
+ qsuff_tac 
+ ‘!l0 x0. Rf(x,t) o Pa(l0,x0) = TRUE ==> P o Pa(l0,x0) = TRUE’ 
+ >-- cheat >>
+ match_mp_tac Rf_min >> arw[] >> 
+ strip_tac (* 2 *)
+ >-- rw[Rf_Nil_unique] >> rpt strip_tac >>
+ drule Rf_Cons_back >> 
+ pop_assum strip_assume_tac >>
+ first_x_assum (qspecl_then [‘a’,‘l’] assume_tac) >> fs[] >>
+ first_x_assum drule >> arw[]                                                            
+ )
+(form_goal
+ “!X x:1->X A t:A * X ->X l0 x0. 
+  Rf(x,t) o Pa(l0,x0) = TRUE ==>
+  !x'. Rf(x,t) o Pa(l0,x') = TRUE ==> x' = x0”));
+
+val List_rec = prove_store("List_rec",
+e0
+()
+(form_goal
+ “!X x:1->X A t:A * X ->X. 
+  ?!f:List(A) -> X. f o Nil(A) = x &
+      f o Cons(A) = t o Pa(p1(A,List(A)), f o p2(A,List(A)))”));
